MemoryModel.thy
@@ -50,6 +50,16 @@ definition empty_memory_model :: "'a memory_model" where
 section "Lemmas"
 
 
+subsection "Simps"
+lemma memory_set_ok_iff[simp]: "valid_memory_address m a \<longleftrightarrow> (\<exists>m'. set_memory m a v = ok m')"
+  unfolding set_memory_def
+  by simp
+
+lemma memory_get_ok_iff[simp]: "valid_memory_address m a \<and> m!a \<noteq> mem_unset \<longleftrightarrow> (\<exists>v. get_memory m a = ok v)"
+  unfolding get_memory_def valid_memory_address_def
+  by (cases "m!a"; simp)
+
+
 
 subsection "Empty"
 
@@ -68,18 +78,11 @@ lemma memory_empty_set: "set_memory empty_memory_model a v = err unallocated_add
 
 subsection "Allocate"
 
-lemma memory_allocate_get_uninitialized: "allocate_memory m = (m', i) \<Longrightarrow> get_memory m' i = err uninitialized_address"
-  unfolding allocate_memory_def get_memory_def
-  apply simp
-  unfolding valid_memory_address_def
+lemma memory_allocate_validity: "allocate_memory m = (m', i) \<Longrightarrow> \<not>valid_memory_address m i \<and> valid_memory_address m' i"
+  unfolding allocate_memory_def valid_memory_address_def
   by auto
 
-
-lemma memory_allocate_validity: "(m', i) = allocate_memory m \<Longrightarrow> \<not>valid_memory_address m i \<and> valid_memory_address m' i"
-  unfolding allocate_memory_def valid_memory_address_def
-  by simp
-
-lemma memory_allocate_independent_valid: "allocate_memory m = (m', a') \<Longrightarrow> a \<noteq> a' \<Longrightarrow> valid_memory_address m a \<longleftrightarrow> valid_memory_address m' a"
+lemma memory_allocate_independent_valid[simp]: "allocate_memory m = (m', a') \<Longrightarrow> a \<noteq> a' \<Longrightarrow> valid_memory_address m a \<longleftrightarrow> valid_memory_address m' a"
   unfolding valid_memory_address_def allocate_memory_def
   using nth_append_left
   by fastforce
@@ -89,6 +92,19 @@ lemma memory_allocate_independent_get: "allocate_memory m = (m', a') \<Longright
   using nth_append_left
   by (cases "a < a'"; fastforce)
 
+lemma memory_allocate_independent_get_wp: "allocate_memory m = (m', a') \<Longrightarrow> a \<noteq> a' \<Longrightarrow> wp_ignore_err (get_memory m' a) (\<lambda>v. ok v = get_memory m a)"
+  unfolding get_memory_def
+  apply simp
+  unfolding valid_memory_address_def allocate_memory_def
+  apply (cases "m'!a"; auto)
+  using allocate_memory_def nth_append_left
+  by (cases "a < a'"; fastforce)
+
+lemma memory_allocate_get_uninitialized: "allocate_memory m = (m', i) \<Longrightarrow> get_memory m' i = err uninitialized_address"
+  unfolding allocate_memory_def get_memory_def
+  apply simp
+  unfolding valid_memory_address_def
+  by auto
 
 subsection "Set"
 
@@ -102,7 +118,7 @@ lemma memory_set_ok_valid: "set_memory m a v = ok m' \<Longrightarrow> valid_mem
   unfolding valid_memory_address_def
   by auto
 
-lemma memory_set_ok_valid_wp: "wp_ok (set_memory m a v) (\<lambda> m'. valid_memory_address m' a \<and> valid_memory_address m a)"
+lemma memory_set_ok_valid_wp: "wp_ignore_err (set_memory m a v) (\<lambda> m'. valid_memory_address m' a \<and> valid_memory_address m a)"
   unfolding set_memory_def
   apply simp
   unfolding valid_memory_address_def
@@ -115,7 +131,7 @@ lemma memory_set_override: "set_memory m i v = ok m' \<Longrightarrow> set_memor
   by auto
 
 lemma memory_set_override_wp:
-  "wp_ok (do {
+  "wp_ignore_err (do {
     m' \<leftarrow> set_memory m a v1;
     m'' \<leftarrow> set_memory m' a v2;
     get_memory m'' a}) (\<lambda>v. v = v2)"
@@ -134,7 +150,7 @@ lemma memory_set_identity: "get_memory m i = ok v \<Longrightarrow> set_memory m
   using list_update_id
   by metis
 
-lemma memory_set_identity_wp: "wp_ok (do { v \<leftarrow> get_memory m a; set_memory m a v }) ((=) m)"
+lemma memory_set_identity_wp: "wp_ignore_err (do { v \<leftarrow> get_memory m a; set_memory m a v }) ((=) m)"
   apply simp
   unfolding get_memory_def set_memory_def
   apply simp
@@ -149,7 +165,7 @@ lemma memory_set_get: "set_memory m i v = ok m' \<Longrightarrow> get_memory m' 
   unfolding valid_memory_address_def
   by auto
 
-lemma memory_set_get_wp: "wp_ok (do {m' \<leftarrow> set_memory m a v; get_memory m' a}) ((=) v)"
+lemma memory_set_get_wp: "wp_ignore_err (do {m' \<leftarrow> set_memory m a v; get_memory m' a}) ((=) v)"
   apply simp
   unfolding set_memory_def get_memory_def
   apply simp
@@ -163,7 +179,7 @@ lemma memory_set_independent_get: "set_memory m a' v = ok m' \<Longrightarrow> a
   unfolding valid_memory_address_def
   by auto
 
-lemma memory_set_independent_get_wp: "a \<noteq> a' \<Longrightarrow> wp_ok (set_memory m a' v) (\<lambda>m'. get_memory m' a = get_memory m a)"
+lemma memory_set_independent_get_wp: "a \<noteq> a' \<Longrightarrow> wp_ignore_err (set_memory m a' v) (\<lambda>m'. get_memory m' a = get_memory m a)"
   unfolding set_memory_def get_memory_def
   apply simp
   unfolding valid_memory_address_def
